mechanization/Compiler/ErgoCompiler.v
@@ -18,7 +18,7 @@ Require ErgoSpec.Version.
 Require ErgoSpec.Backend.ErgoBackend.
 Require ErgoSpec.Common.Utils.ENames.
 Require ErgoSpec.Common.Utils.EResult.
-Require ErgoSpec.Common.Utils.EImport.
+Require ErgoSpec.Common.Utils.EAstUtil.
 Require ErgoSpec.Common.CTO.CTO.
 Require ErgoSpec.Common.Types.ErgoType.
 Require ErgoSpec.Common.Pattern.EPattern.
@@ -35,101 +35,115 @@ Module ErgoCompiler.
   Module ErgoData := ErgoBackend.ErgoData.
   Module ErgoOps := ErgoBackend.ErgoOps.
 
+  (** Utils *)
+  (* XXX Exposed so it can be called from JavaScript - Should be removed once we switch to the REPL *)
+  Definition javascript_identifier_sanitizer := ErgoBackend.ErgoCodeGen.javascript_identifier_sanitizer.
+  
+  (** Location *)
+  Definition location := EResult.location.
+
   (** Names *)
-  Definition name_ref : Set
-    := ENames.name_ref.
-  Definition mk_relative_ref : option String.string -> String.string -> name_ref
-    := ENames.RelativeRef.
-  Definition mk_absolute_ref : String.string -> name_ref
-    := ENames.AbsoluteRef.
+  Definition relative_name : Set := ENames.relative_name.
 
   (** CTOs *)
-  Definition cto_boolean loc : CTO.cto_type
-    := CTO.mk_cto loc CTO.CTOBoolean.
-  Definition cto_string loc : CTO.cto_type
-    := CTO.mk_cto loc CTO.CTOString.
-  Definition cto_double loc : CTO.cto_type
-    := CTO.mk_cto loc CTO.CTODouble.
-  Definition cto_long loc : CTO.cto_type
-    := CTO.mk_cto loc CTO.CTOLong.
-  Definition cto_integer loc : CTO.cto_type
-    := CTO.mk_cto loc CTO.CTOInteger.
-  Definition cto_dateTime loc : CTO.cto_type
-    := CTO.mk_cto loc CTO.CTODateTime.
-  Definition cto_class_ref loc name_ref : CTO.cto_type
-    := CTO.mk_cto loc (CTO.CTOClassRef name_ref).
-  Definition cto_option loc ct : CTO.cto_type
-    := CTO.mk_cto loc (CTO.CTOOption ct).
-  Definition cto_array loc ct : CTO.cto_type
-    := CTO.mk_cto loc (CTO.CTOArray ct).
+  Definition cto_type := CTO.lrcto_type.
+  Definition cto_declaration_desc := CTO.lrcto_declaration_desc.
+  Definition cto_declaration := CTO.lrcto_declaration.
+  Definition cto_package := CTO.lrcto_package.
+  
+  Definition cto_boolean : location -> cto_type
+    := CTO.CTOBoolean.
+  Definition cto_string : location -> cto_type
+    := CTO.CTOString.
+  Definition cto_double : location -> cto_type
+    := CTO.CTODouble.
+  Definition cto_long : location -> cto_type
+    := CTO.CTOLong.
+  Definition cto_integer : location -> cto_type
+    := CTO.CTOInteger.
+  Definition cto_dateTime : location -> cto_type
+    := CTO.CTODateTime.
+  Definition cto_class_ref loc name_ref : cto_type
+    := CTO.CTOClassRef loc name_ref.
+  Definition cto_option loc ct : cto_type
+    := CTO.CTOOption loc ct.
+  Definition cto_array loc ct : cto_type
+    := CTO.CTOArray loc ct.
 
-  Definition cto_enum : list String.string -> CTO.cto_declaration_desc
+  Definition cto_enum : list String.string -> cto_declaration_desc
     := CTO.CTOEnum.
-  Definition cto_transaction : option name_ref -> list (String.string * CTO.cto_type) -> CTO.cto_declaration_desc
+  Definition cto_transaction : option relative_name -> list (String.string * cto_type) -> cto_declaration_desc
     := CTO.CTOTransaction.
-  Definition cto_concept : option name_ref -> list (String.string * CTO.cto_type) -> CTO.cto_declaration_desc
+  Definition cto_concept : option relative_name -> list (String.string * cto_type) -> cto_declaration_desc
     := CTO.CTOConcept.
 
-  Definition mk_cto_declaration : String.string -> EResult.location -> CTO.cto_declaration_desc -> CTO.cto_declaration
+  Definition mk_cto_declaration : EResult.location -> String.string -> cto_declaration_desc -> cto_declaration
     := CTO.mkCTODeclaration.
-  Definition mk_cto_package : String.string -> EResult.location -> list EImport.import_decl -> list CTO.cto_declaration -> CTO.cto_package
+  Definition mk_cto_package : EResult.location -> String.string -> list EAstUtil.import_decl -> list cto_declaration -> cto_package
     := CTO.mkCTOPackage.
 
   (** Types *)
-  Definition ergo_type : Set 
-    := ErgoType.ergo_type.
+  Definition ergo_type : Set
+    := ErgoType.lrergo_type.
+  Definition ergo_type_declaration_desc : Set :=
+    ErgoType.lrergo_type_declaration_desc.
+  Definition ergo_type_declaration : Set :=
+    ErgoType.lrergo_type_declaration.
+  Definition ergo_type_module : Set :=
+    ErgoType.lrergo_type_module.
+  
   Definition ergo_type_any loc : ergo_type
-    := ErgoType.mk_type loc ErgoType.ErgoTypeAny.
+    := ErgoType.ErgoTypeAny loc.
   Definition ergo_type_none loc : ergo_type
-    := ErgoType.mk_type loc ErgoType.ErgoTypeNone.
+    := ErgoType.ErgoTypeNone loc.
   Definition ergo_type_boolean loc : ergo_type
-    := ErgoType.mk_type loc ErgoType.ErgoTypeBoolean.
+    := ErgoType.ErgoTypeBoolean loc.
   Definition ergo_type_string loc : ergo_type
-    := ErgoType.mk_type loc ErgoType.ErgoTypeString.
+    := ErgoType.ErgoTypeString loc.
   Definition ergo_type_double loc : ergo_type
-    := ErgoType.mk_type loc ErgoType.ErgoTypeDouble.
+    := ErgoType.ErgoTypeDouble loc.
   Definition ergo_type_long loc : ergo_type
-    := ErgoType.mk_type loc ErgoType.ErgoTypeLong.
+    := ErgoType.ErgoTypeLong loc.
   Definition ergo_type_integer loc : ergo_type
-    := ErgoType.mk_type loc ErgoType.ErgoTypeInteger.
+    := ErgoType.ErgoTypeInteger loc.
   Definition ergo_type_dateTime loc : ergo_type
-    := ErgoType.mk_type loc ErgoType.ErgoTypeDateTime.
-  Definition ergo_type_class_ref loc name_ref : ergo_type
-    := ErgoType.mk_type loc (ErgoType.ErgoTypeClassRef name_ref).
+    := ErgoType.ErgoTypeDateTime loc.
+  Definition ergo_type_class_ref loc relative_name : ergo_type
+    := ErgoType.ErgoTypeClassRef loc relative_name.
   Definition ergo_type_option loc et : ergo_type
-    := ErgoType.mk_type loc (ErgoType.ErgoTypeOption et).
+    := ErgoType.ErgoTypeOption loc et.
   Definition ergo_type_record loc rec : ergo_type
-    := ErgoType.mk_type loc (ErgoType.ErgoTypeRecord rec).
+    := ErgoType.ErgoTypeRecord loc rec.
   Definition ergo_type_array loc et : ergo_type
-    := ErgoType.mk_type loc (ErgoType.ErgoTypeArray et).
+    := ErgoType.ErgoTypeArray loc et.
 
-  Definition ergo_type_enum : list String.string -> ErgoType.ergo_type_declaration_desc
+  Definition ergo_type_enum : list String.string -> ergo_type_declaration_desc
     := ErgoType.ErgoTypeEnum.
-  Definition ergo_type_transaction : option name_ref -> list (String.string * ErgoType.ergo_type) -> ErgoType.ergo_type_declaration_desc
+  Definition ergo_type_transaction : option relative_name -> list (String.string * ergo_type) -> ergo_type_declaration_desc
     := ErgoType.ErgoTypeTransaction.
-  Definition ergo_type_concept : option name_ref -> list (String.string * ErgoType.ergo_type) -> ErgoType.ergo_type_declaration_desc
+  Definition ergo_type_concept : option relative_name -> list (String.string * ergo_type) -> ergo_type_declaration_desc
     := ErgoType.ErgoTypeConcept.
 
-  Definition mk_ergo_type_declaration : String.string -> EResult.location -> ErgoType.ergo_type_declaration_desc -> ErgoType.ergo_type_declaration
+  Definition mk_ergo_type_declaration : EResult.location -> String.string -> ergo_type_declaration_desc -> ergo_type_declaration
     := ErgoType.mkErgoTypeDeclaration.
-  Definition mk_ergo_type_module : String.string -> EResult.location -> list EImport.import_decl -> list ErgoType.ergo_type_declaration -> ErgoType.ergo_type_module
+  Definition mk_ergo_type_module : EResult.location -> String.string -> list EAstUtil.import_decl -> list ergo_type_declaration -> ergo_type_module
     := ErgoType.mkErgoTypeModule.
 
   (** Ergo *)
   Definition ergo_expr : Set 
-    := Ergo.ergo_expr.
+    := Ergo.lrergo_expr.
   Definition ergo_stmt : Set 
-    := Ergo.ergo_stmt.
+    := Ergo.lrergo_stmt.
   Definition ergo_function : Set
-    := Ergo.ergo_function.
+    := Ergo.lrergo_function.
   Definition ergo_clause : Set
-    := Ergo.ergo_clause.
+    := Ergo.lrergo_clause.
   Definition ergo_declaration : Set
-    := Ergo.ergo_declaration.
-  Definition ergo_module : Set 
-    := Ergo.ergo_module.
+    := Ergo.lrergo_declaration.
   Definition ergo_contract : Set
-    := Ergo.ergo_contract.
+    := Ergo.lrergo_contract.
+  Definition ergo_module : Set 
+    := Ergo.lrergo_module.
 
   (** Patterns *)
   Definition ecasedata : ErgoData.data -> EPattern.ergo_pattern
@@ -143,59 +157,59 @@ Module ErgoCompiler.
 
   (** Expressions *)
   Definition ethis_contract loc : ergo_expr
-    := Ergo.mk_expr loc Ergo.EThisContract.
+    := Ergo.EThisContract loc.
   Definition ethis_clause loc : ergo_expr
-    := Ergo.mk_expr loc Ergo.EThisClause.
+    := Ergo.EThisClause loc.
   Definition ethis_state loc : ergo_expr
-    := Ergo.mk_expr loc Ergo.EThisState.
+    := Ergo.EThisState loc.
   Definition evar loc v: ergo_expr
-    := Ergo.mk_expr loc (Ergo.EVar v).
+    := Ergo.EVar loc v.
   Definition econst loc d :ergo_expr
-    := Ergo.mk_expr loc (Ergo.EConst d).
+    := Ergo.EConst loc d.
   Definition earray loc arr : ergo_expr
-    := Ergo.mk_expr loc (Ergo.EArray arr).
+    := Ergo.EArray loc arr.
   Definition eunaryop loc u e : ergo_expr
-    := Ergo.mk_expr loc (Ergo.EUnaryOp u e).
+    := Ergo.EUnaryOp loc u e.
   Definition ebinaryop loc b e1 e2 : ergo_expr 
-    := Ergo.mk_expr loc (Ergo.EBinaryOp b e1 e2).
+    := Ergo.EBinaryOp loc b e1 e2.
   Definition eif loc e1 e2 e3 : ergo_expr 
-    := Ergo.mk_expr loc (Ergo.EIf e1 e2 e3).
+    := Ergo.EIf loc e1 e2 e3.
   Definition elet loc (v:String.string) (t:option ErgoType.ergo_type) (e1 e2:ergo_expr) : ergo_expr
-    := Ergo.mk_expr loc (Ergo.ELet v t e1 e2).
+    := Ergo.ELet loc v t e1 e2.
   Definition enew loc n rec : ergo_expr 
-    := Ergo.mk_expr loc (Ergo.ENew n rec).
+    := Ergo.ENew loc n rec.
   Definition erecord loc rec : ergo_expr 
-    := Ergo.mk_expr loc (Ergo.ERecord rec).
+    := Ergo.ERecord loc rec.
   Definition ecallfun loc f el : ergo_expr
-    := Ergo.mk_expr loc (Ergo.ECallFun f el).
+    := Ergo.ECallFun loc f el.
   Definition ematch loc e0 epl ed : ergo_expr
-    := Ergo.mk_expr loc (Ergo.EMatch e0 epl ed).
+    := Ergo.EMatch loc e0 epl ed.
   Definition eforeach loc efl ew er : ergo_expr
-    := Ergo.mk_expr loc (Ergo.EForeach efl ew er).
+    := Ergo.EForeach loc efl ew er.
 
   (** Statements *)
   Definition sreturn loc e : ergo_stmt :=
-    Ergo.mk_stmt loc (Ergo.SReturn e).
+    Ergo.SReturn loc e.
   Definition sfunreturn loc e : ergo_stmt :=
-    Ergo.mk_stmt loc (Ergo.SFunReturn e).
+    Ergo.SFunReturn loc e.
   Definition sthrow loc e : ergo_stmt :=
-    Ergo.mk_stmt loc (Ergo.SThrow e).
+    Ergo.SThrow loc e.
   Definition scallclause loc c el : ergo_stmt :=
-    Ergo.mk_stmt loc (Ergo.SCallClause c el).
+    Ergo.SCallClause loc c el.
   Definition ssetstate loc e s : ergo_stmt :=
-    Ergo.mk_stmt loc (Ergo.SSetState  e s).
+    Ergo.SSetState loc e s.
   Definition semit loc e s : ergo_stmt :=
-    Ergo.mk_stmt loc (Ergo.SEmit e s).
+    Ergo.SEmit loc e s.
   Definition slet loc (v:String.string) (e1:ergo_expr) (s2:ergo_stmt) : ergo_stmt :=
-    Ergo.mk_stmt loc (Ergo.SLet v None e1 s2).
+    Ergo.SLet loc v None e1 s2.
   Definition slet_typed loc (v:String.string) (t:ErgoType.ergo_type) (e1:ergo_expr) (s2:ergo_stmt) : ergo_stmt :=
-    Ergo.mk_stmt loc (Ergo.SLet v (Some t) e1 s2).
+    Ergo.SLet loc v (Some t) e1 s2.
   Definition sif loc e1 s2 s3 : ergo_stmt :=
-    Ergo.mk_stmt loc (Ergo.SIf e1 s2 s3).
+    Ergo.SIf loc e1 s2 s3.
   Definition senforce loc (e1:ergo_expr) (s2: option ergo_stmt) (s3:ergo_stmt) : ergo_stmt :=
-    Ergo.mk_stmt loc (Ergo.SEnforce e1 s2 s3).
+    Ergo.SEnforce loc e1 s2 s3.
   Definition smatch loc e slp sd : ergo_stmt :=
-    Ergo.mk_stmt loc (Ergo.SMatch e slp sd).
+    Ergo.SMatch loc e slp sd.
 
   (** Syntactic sugar *)
   Definition edot : EResult.location -> String.string -> ergo_expr -> ergo_expr 
@@ -211,15 +225,15 @@ Module ErgoCompiler.
   
   (** Declarations *)
   Definition dtype loc etd : ergo_declaration
-    := Ergo.mk_decl loc (Ergo.DType etd).
+    := Ergo.DType loc etd.
   Definition dstmt loc s : ergo_declaration
-    := Ergo.mk_decl loc (Ergo.DStmt s).
+    := Ergo.DStmt loc s.
   Definition dconstant loc v e : ergo_declaration
-    := Ergo.mk_decl loc (Ergo.DConstant v e).
+    := Ergo.DConstant loc v e.
   Definition dfunc loc f : ergo_declaration
-    := Ergo.mk_decl loc (Ergo.DFunc f).
+    := Ergo.DFunc loc f.
   Definition dcontract loc c : ergo_declaration
-    := Ergo.mk_decl loc (Ergo.DContract c).
+    := Ergo.DContract loc c.
 
   (** Compilation *)
   Definition ergo_module_to_javascript :
