mechanization/Backend/Lib/EData.v
@@ -78,6 +78,7 @@ Module EData(ergomodel:ErgoBackendModel).
   (** data -> JSON *string* conversion *)
   Definition data_to_json_string s : Data.data -> String.string 
     := ergomodel.ergo_data_to_json_string s.
+
   Definition json_to_json_string s : json -> String.string 
     := JSON.jsonToJS s.
 
