mechanization/Ergo/Lang/ErgoSugar.v
@@ -25,75 +25,78 @@ Require Import ErgoSpec.Ergo.Lang.Ergo.
 Require Import ErgoSpec.Backend.ErgoBackend.
 
 Section ErgoSugar.
-  (** [expr.field] is a macro for unbranding followed by field access in a record *)
-  Definition EDot (loc:location) (s:string) (e:ergo_expr) : ergo_expr :=
-    mk_expr loc (EUnaryOp (ErgoOps.Unary.opdot s)
-                          (mk_expr loc (EUnaryOp ErgoOps.Unary.opunbrand e))).
-
-  (** [return expr] is a no-op at the moment *)
-  Definition mk_result (loc:location) e1 e2 e3 : ergo_expr :=
-    mk_expr loc
-            (ERecord ((this_response, e1)
-                        :: (this_state, e2)
-                        :: (this_emit, e3)
-                        :: nil)).
-
-  Definition set_state (loc:location) e1 e2 : ergo_expr :=
-    mk_expr loc
-            (ELet local_state None e1 e2).
-
-  Definition this_clause (loc:location) clause_name :=
-    mk_expr loc
-            (EUnaryOp (OpDot clause_name)
-                      (mk_expr loc (EUnaryOp OpUnbrand (mk_expr loc EThisContract)))).
-
-  Definition push_emit (loc:location) e1 e2 : ergo_expr :=
-    mk_expr loc
-            (ELet local_emit None
-                  (mk_expr loc
-                           (EBinaryOp OpBagUnion
-                                      (mk_expr loc (EUnaryOp OpBag e1))
-                                      (mk_expr loc (EVar local_emit))))
-                  e2).
-
-  Definition SThrowSugar (loc:location) pname cname el : ergo_stmt :=
-    mk_stmt loc
-            (SThrow (mk_expr loc (ENew (RelativeRef pname cname) el))).
-
-  Definition SThrowErgoCompilerError (loc:location) (msg:string) : ergo_stmt :=
-    SThrowSugar loc
-                (Some "org.ergo"%string)
-                "Error"%string
-                (("error"%string, mk_expr loc
-                                   (EConst (ErgoData.dstring msg)))::nil).
-
-  Definition SReturnEmpty (loc:location) :=
-    mk_stmt loc (SReturn (mk_expr loc (EConst dunit))).
+  Section ParserSugar.
+    Context {A:Set}. (* Type for annotations *)
   
-  Definition SFunReturnEmpty (loc:location) :=
-    mk_stmt loc (SFunReturn (mk_expr loc (EConst dunit))).
+    (** [expr.field] is a macro for unbranding followed by field access in a record *)
+    Definition EDot (a:A) (s:string) (e:rergo_expr) : rergo_expr :=
+      EUnaryOp a
+               (ErgoOps.Unary.opdot s)
+               (EUnaryOp a ErgoOps.Unary.opunbrand e).
 
-  Section Errors.
-    Definition ESuccess (loc:location) (e:ergo_expr) : ergo_expr :=
-      mk_expr loc (EUnaryOp OpLeft e).
+    Definition SReturnEmpty (a:A) : rergo_stmt :=
+      SReturn a (EConst a dunit).
+  
+    Definition SFunReturnEmpty (a:A) : rergo_stmt :=
+      SFunReturn a (EConst a dunit).
+
+    Definition EOptionalDot (a:A) (pname:string) (e:rergo_expr) :=
+      EMatch a
+             e
+             ((CaseLetOption "$option" None,
+               EUnaryOp a (OpDot pname) (EVar a "$option")) :: nil)
+             (EConst a dnone).
+    Definition EOptionalDefault (a:A) (e1 e2:rergo_expr) :=
+      EMatch a e1
+             ((CaseLetOption "$option" None, EVar a "$option") :: nil)
+             e2.
+
+    (*
+    Definition SThrowSugar (loc:location) (ns:namespace_prefix) (ln:local_name) (el:list (string*laergo_expr)) : laergo_stmt :=
+      SThrow loc (ENew loc (ns,ln) el).
+*)
+
+    (*
+    Definition SThrowErgoCompilerError (a:A) (msg:string) : rergo_stmt :=
+      SThrowSugar a
+                  (Some "org.ergo"%string)
+                  "Error"%string
+                  (("error"%string, EConst a (ErgoData.dstring msg))::nil).
+*)
+
+  End ParserSugar.
+
+  Section StmtSugar.
+    (** [return expr] is a no-op at the moment *)
+    Definition mk_result (loc:location) e1 e2 e3 : laergo_expr :=
+      ERecord loc
+              ((this_response, e1)
+                 :: (this_state, e2)
+                 :: (this_emit, e3)
+                 :: nil).
+
+    Definition set_state (loc:location) e1 e2 : laergo_expr :=
+      ELet loc local_state None e1 e2.
+
+    Definition this_clause (loc:location) clause_name : laergo_expr :=
+      EUnaryOp loc
+               (OpDot clause_name)
+               (EUnaryOp loc OpUnbrand (EThisContract loc)).
+
+    Definition push_emit (loc:location) e1 e2 : laergo_expr :=
+      ELet loc local_emit None
+           (EBinaryOp loc
+                      OpBagUnion
+                      (EUnaryOp loc OpBag e1)
+                      (EVar loc local_emit))
+           e2.
+
+    Definition ESuccess (loc:location) (e:laergo_expr) : laergo_expr :=
+      EUnaryOp loc OpLeft e.
       
-    Definition EError (loc:location) (e:ergo_expr) : ergo_expr :=
-      mk_expr loc (EUnaryOp OpRight e).
+    Definition EError (loc:location) (e:laergo_expr) : laergo_expr :=
+      EUnaryOp loc OpRight e.
 
-  End Errors.
-
-  Section Optional.
-    Definition EOptionalDot (loc:location) (pname:string) (e:ergo_expr) :=
-      mk_expr loc
-              (EMatch e
-                      ((CaseLetOption "$option" None,
-                        mk_expr loc (EUnaryOp (OpDot pname) (mk_expr loc (EVar "$option")))) :: nil)
-                      (mk_expr loc (EConst dnone))).
-    Definition EOptionalDefault (loc:location) (e1 e2:ergo_expr) :=
-      mk_expr loc
-              (EMatch e1
-                      ((CaseLetOption "$option" None, mk_expr loc (EVar "$option")) :: nil)
-                      e2).
-  End Optional.
+  End StmtSugar.
 
 End ErgoSugar.
