mechanization/Translation/ErgoNNRCtoJavaScriptCicero.v
@@ -79,7 +79,7 @@ Section ErgoNNRCtoJavaScriptCicero.
       ++ "function " ++ fun_name ++ "(context) {" ++ eol
       ++ "  let pcontext = { 'request' : serializer.toJSON(context.request,{permitResourcesForRelationships:true}), 'state': " ++ state_init ++ ", 'contract': serializer.toJSON(context.contract,{permitResourcesForRelationships:true}), 'emit': context.emit, 'now': context.now};" ++ eol
       ++ "  //logger.info('ergo context: '+JSON.stringify(pcontext))" ++ eol
-      ++ "  let result = new " ++ contract_name ++ "()." ++ clause_name ++ "(pcontext);" ++ eol
+      ++ "  let result = new " ++ ErgoCodeGen.javascript_identifier_sanitizer contract_name ++ "()." ++ ErgoCodeGen.javascript_identifier_sanitizer clause_name ++ "(pcontext);" ++ eol
       ++ "  if (result.hasOwnProperty('left')) {" ++ eol
       ++ "    //logger.info('ergo result: '+JSON.stringify(result))" ++ eol
       ++ "    context.response = serializer.fromJSON(result.left.response, {validate: false, acceptResourcesForRelationships: true},{permitResourcesForRelationships:true});" ++ eol
@@ -102,7 +102,7 @@ Section ErgoNNRCtoJavaScriptCicero.
              (eol:string)
              (quotel:string) : ErgoCodeGen.javascript :=
     let '(clause_name, request_type, response_type, emit_type) := signature in
-    let fun_name := contract_name ++ "_" ++ clause_name in
+    let fun_name := ErgoCodeGen.javascript_identifier_sanitizer contract_name ++ "_" ++ ErgoCodeGen.javascript_identifier_sanitizer clause_name in
     wrapper_function
       fun_name request_type response_type emit_type contract_state_type contract_name clause_name eol quotel.
   
@@ -130,32 +130,29 @@ Section ErgoNNRCtoJavaScriptCicero.
                    ++ (javascript_of_declarations p.(modulen_declarations) 0 0 eol quotel)
                    ++ (postamble eol).
 
-  Fixpoint filter_signatures (namespace:string) (sigs:list ergo_type_signature) : list (string * string * string * string) :=
+  Fixpoint filter_signatures
+           (namespace:string)
+           (sigs:list (string * laergo_type_signature))
+    : list (string * string * string * string) :=
     match sigs with
     | nil => nil
-    | sig :: rest =>
-      if (string_dec sig.(type_signature_name) clause_main_name)
+    | (fname,sig) :: rest =>
+      if (string_dec fname clause_main_name)
       then
         filter_signatures namespace rest
       else
-        let fname := sig.(type_signature_name) in
         let params := sig.(type_signature_params) in
         let outtype := sig.(type_signature_output) in
         let emitstype := sig.(type_signature_emits) in
         match params with
         | nil => filter_signatures namespace rest
         | (_,reqtype)::nil =>
-          match type_desc reqtype, type_desc outtype, lift type_desc emitstype with
-          | ErgoTypeClassRef reqname, ErgoTypeClassRef outname, Some (ErgoTypeClassRef emitsname) =>
-            let qreqname := absolute_name_of_name_ref namespace reqname in
-            let qoutname := absolute_name_of_name_ref namespace outname in
-            let qemitsname := absolute_name_of_name_ref namespace emitsname in
-            (fname,qreqname,qoutname,qemitsname) :: (filter_signatures namespace rest)
-          | ErgoTypeClassRef reqname, ErgoTypeClassRef outname, None =>
-            let qreqname := absolute_name_of_name_ref namespace reqname in
-            let qoutname := absolute_name_of_name_ref namespace outname in
-            let qemitsname := default_emits_name in
-            (fname,qreqname,qoutname,qemitsname) :: (filter_signatures namespace rest)
+          match reqtype, outtype, emitstype with
+          | ErgoTypeClassRef _ reqname, ErgoTypeClassRef _ outname, Some (ErgoTypeClassRef _ emitsname) =>
+            (fname,reqname,outname,emitsname) :: (filter_signatures namespace rest)
+          | ErgoTypeClassRef _ reqname, ErgoTypeClassRef _ outname, None =>
+            let emitsname := default_emits_absolute_name in
+            (fname,reqname,outname,emitsname) :: (filter_signatures namespace rest)
           | _, _, _ =>
             filter_signatures namespace rest
           end
@@ -163,12 +160,15 @@ Section ErgoNNRCtoJavaScriptCicero.
         end
     end.
 
-  Definition filter_signatures_with_state (namespace:string) (contract_state_type:option ergo_type) (sigs:list ergo_type_signature) : list (string * string * string * string) * string :=
-    match lift type_desc contract_state_type with
-    | None => (filter_signatures namespace sigs, default_state_name)
-    | Some (ErgoTypeClassRef statename) =>
-      let qstatename := absolute_name_of_name_ref namespace statename in
-      (filter_signatures namespace sigs, qstatename)
+  Definition filter_signatures_with_state
+             (namespace:string)
+             (contract_state_type:option laergo_type)
+             (sigs:list (string * ergo_type_signature))
+    : list (string * string * string * string) * string :=
+    match contract_state_type with
+    | None => (filter_signatures namespace sigs, default_state_absolute_name)
+    | Some (ErgoTypeClassRef _ statename) =>
+      (filter_signatures namespace sigs, statename)
     | _ =>
       (nil, "")
     end.
@@ -176,7 +176,7 @@ Section ErgoNNRCtoJavaScriptCicero.
   Definition ergoc_module_to_javascript_cicero
              (contract_name:string)
              (contract_state_type:option ergo_type)
-             (sigs: list ergo_type_signature)
+             (sigs: list (string * ergo_type_signature))
              (p:nnrc_module) : ErgoCodeGen.javascript :=
     javascript_of_module_with_dispatch
       contract_name
